coq-osiris/theories/base.v
@@ -1,5 +1,8 @@
 Require Export Coq.Program.Equality.
 From stdpp Require Export base strings.
+From osiris.logic Require Export void.
+
+(* TODO move all of the following to other places? *)
 
 (* Logical tautologies. *)
 
