coq-osiris/theories/logic/void.v
@@ -1,0 +1,9 @@
+(* The empty type and its elimination form. *)
+
+Definition void : Type := Empty_set.
+
+Definition elim_void {A} (v : void) : A :=
+  match v with end.
+
+Ltac elim_void e :=
+  exfalso; exact (elim_void e).
